ameliorations

Lib.v
@@ -2,39 +2,63 @@
 Set Implicit Arguments.
 Unset Strict Implicit.
 Unset Printing Implicit Defensive.
-(* Vec {A} B l is a B-list of the same size as l *)
-Inductive Vec {A : Type} (B : Type) : list A -> Type :=
-    NilV : Vec B nil
-  | ConsV : forall a lA, B -> Vec B lA -> Vec B (a :: lA).
 
-Definition Vec_map {A B C : Type}(f : A -> B -> C) :=
-  fix rec (l : list A) (v : Vec B l) : Vec C l :=
+(* vec {A} B l is a B-list of the same size as l *)
+Inductive vec {A : Type} (B : Type) : list A -> Type :=
+    NilV : vec B nil
+  | ConsV : forall a lA, B -> vec B lA -> vec B (a :: lA).
+
+Arguments NilV {A}{B}.
+
+Definition vec_hd {A B}(a : A)(l : list A)(v : vec B (a :: l)) : B :=
+  match v with ConsV _ b _ => b end.
+Definition vec_tl {A B}(a : A)(l : list A)(v : vec B (a :: l)) : vec B l :=
+  match v with ConsV _ _ v => v end.
+
+  
+Declare Scope vec_scope.
+Delimit Scope vec_scope with v.
+
+Infix "::" := (ConsV _) (only parsing) : vec_scope.
+
+Definition vec_map {A B C : Type}(f : A -> B -> C) :=
+  fix rec (l : list A) (v : vec B l) : vec C l :=
   match v with
-    NilV _ => NilV _
+    NilV => NilV
   | ConsV a b lB => ConsV a (f a b) (rec _ lB)
     end.
 
-Fixpoint Vec_map_id {A B : Type}{l : list A}(v : Vec B l) : Vec_map (fun _ x => x) v = v.
+Definition vec_hd_map  {A B C}(a : A)(l : list A)(f : A -> B -> C)
+                          (v : vec B (a :: l)) :
+                         vec_hd (vec_map f v) = f a (vec_hd v) :=
+  match v with ConsV _ b v' => eq_refl _ end.
+
+Definition vec_tl_map  {A B C}(a : A)(l : list A)(f : A -> B -> C)
+                          (v : vec B (a :: l)) :
+                         vec_tl (vec_map f v) = vec_map f (vec_tl v) :=
+  match v with ConsV _ b v' => eq_refl _ end.
+
+Fixpoint vec_map_id {A B : Type}{l : list A}(v : vec B l) : vec_map (fun _ x => x) v = v.
   destruct v.
   -  reflexivity.
   -  cbn.
      f_equal.
-     apply Vec_map_id.
+     apply vec_map_id.
 Defined.
 
 Lemma vec_map_map {A B C D : Type}(f : A -> B -> C) (g : A -> C -> D) {l : list A}
-      (v : Vec B l) : Vec_map g (Vec_map f v) = Vec_map (fun a b => g a (f a b)) v.
+      (v : vec B l) : vec_map g (vec_map f v) = vec_map (fun a b => g a (f a b)) v.
   induction v; cbn; congruence.
 Qed.
 
 Definition vec_map_ext {A B C : Type}(f g : A -> B -> C) {l : list A}
-      (v : Vec B l) (h : forall a b, f a b = g a b): Vec_map f v = Vec_map g v.
+      (v : vec B l) (h : forall a b, f a b = g a b): vec_map f v = vec_map g v.
   induction v; cbn; congruence.
 Defined.
 
-Fixpoint vec_max {A : Type}(l : list A) (v : Vec nat l) : nat :=
+Fixpoint vec_max {A : Type}(l : list A) (v : vec nat l) : nat :=
   match v with
-    NilV _ => 0
+    NilV => 0
   | ConsV a b lB => Nat.max b (vec_max lB)
     end.
 
