Quot.v
@@ -26,21 +26,20 @@ Record Eqv (X : Type) : Type := {
     eqv_data x y -> eqv_data y z -> eqv_data x z
 }.
 
-Hint Immediate eqv_sym.
-Hint Resolve eqv_rfl eqv_trs.
 
 Lemma eq_eqv : forall X (r : Eqv X) x y, x = y -> r x y.
 Proof.
 destruct 1. apply eqv_rfl.
 Qed.
 
-Hint Resolve eq_eqv.
-
 
 (** ** Quotients *)
 
 Parameter quotient : forall (X : Type) (r : Eqv X), Type.
 Arguments quotient : clear implicits.
+
+Declare Scope quotient.
+
 Infix "//" := quotient
   (at level 45, right associativity) : quotient.
 Open Scope quotient.
@@ -51,11 +50,9 @@ Notation "x / r" := (class r x) : quotient.
 
 Axiom class_eq : forall (X : Type) (r : Eqv X) (x y : X),
   r x y -> x/r = y/r.
-Hint Resolve class_eq.
 
 Axiom class_rel : forall (X : Type) (r : Eqv X) (x y : X),
   x/r = y/r -> r x y.
-Hint Resolve class_rel.
 
 Axiom class_ind : forall (X : Type) (r : Eqv X) (P : X // r -> Prop),
   (forall x : X, P (x / r)) -> forall x : X // r, P x.
@@ -68,8 +65,6 @@ Arguments factor [X] r [Y].
 Axiom factorize : forall (X : Type) (r : Eqv X) (Y : Type) (f : X -> Y)
   (H : forall x y, r x y -> f x = f y),
     forall x ,  factor r f H (x/r) = f x.
-Hint Resolve factorize.
-Hint Rewrite factorize : quotient.
 
 Lemma factor_extens : forall X (r : Eqv X) Y (f g : X -> Y)
   (Hf : forall x y, r x y -> f x = f y)
@@ -83,29 +78,6 @@ intros.
 do 2 rewrite factorize. trivial.
 Qed.
 
-Definition frel X Y (r : Eqv Y) (f g : X -> Y) : Prop :=
-  forall x, r (f x) (g x).
-
-Definition feqv X Y (r : Eqv Y) : Eqv (X -> Y).
-Proof.
-intros.
-split with (@frel X Y r);
-  abstract (unfold frel; simpl; trivial; firstorder eauto).
-Defined.
-
-Definition theta' X Y (r : Eqv Y) : (X -> Y) -> (X -> Y // r) :=
-  fun f x => f x / r.
-
-Lemma theta'_compat : forall  X Y (r : Eqv Y) (f g : X -> Y),
-  feqv X r f g -> theta' r f = theta' r g.
-Proof.
-simpl. intros. unfold theta'.
-apply extensionality. auto.
-Qed.
-
-Definition theta X Y (r : Eqv Y) : (X -> Y) // feqv X r -> X -> Y // r :=
-  fun (f : (X -> Y) // feqv X r) (x : X) =>
-    factor (feqv X r) (@theta' X Y r) (@theta'_compat X Y r) f x.
 
 
 Section Factor1.
@@ -116,7 +88,7 @@ Hypothesis Hf : forall x y, rX x y -> rY (f x) (f y).
 Definition factor1 : X // rX -> Y // rY.
 Proof.
 apply (factor rX (fun x => f x / rY)).
-abstract auto.
+abstract auto using class_eq.
 Defined.
 
 Lemma factorize1 : forall x, factor1 (x / rX) = f x / rY.
@@ -129,7 +101,6 @@ End Factor1.
 
 Arguments factor1 [X] rX [Y].
 Arguments factorize1 [X] rX [Y] rY.
-Hint Rewrite factorize1 : quotient.
 
 Lemma factor1_extens : forall X (rX : Eqv X) Y (rY : Eqv Y) (f g : X -> Y)
   (Hf : forall x y, rX x y -> rY (f x) (f y))
@@ -138,7 +109,7 @@ Lemma factor1_extens : forall X (rX : Eqv X) Y (rY : Eqv Y) (f g : X -> Y)
   forall x, factor1 rX rY f Hf x = factor1 rX rY g Hg x.
 Proof.
 intros. unfold factor1.
-apply factor_extens. auto.
+apply factor_extens. auto using class_eq.
 Qed.
 
 Section Factor2.
@@ -151,7 +122,7 @@ Hypothesis Hf : forall x y z w,
 
 Let h  (x : X) : Y // rY -> Z // rZ.
 Proof.
-intro. apply (factor1 rY rZ (f x)). abstract auto.
+intro. apply (factor1 rY rZ (f x)). abstract auto using eqv_rfl.
 assumption.
 Defined.
 
@@ -162,7 +133,7 @@ apply (class_ind
   (fun x0 =>
     factor1 rY rZ (f x) (h_subproof x) x0 = factor1 rY rZ (f y) (h_subproof y) x0)).
 intros.
-do 2 rewrite factorize1. auto.
+do 2 rewrite factorize1. auto using class_eq, eqv_rfl.
 Qed.
 
 Definition factor2 : X // rX -> Y // rY -> Z // rZ.
@@ -182,7 +153,6 @@ End Factor2.
 Arguments factor2 [X] _ [Y] _ [Z].
 Arguments factorize2 [X] _ [Y] _ [Z].
 
-Hint Rewrite factorize2 : quotient.
 
 Lemma factor2_extens :
   forall X (rX : Eqv X) Y (rY : Eqv Y) Z (rZ : Eqv Z)
@@ -200,7 +170,7 @@ apply (class_ind
 intro.
 apply (class_ind
   (fun y => factor2 rX rY rZ f Hf (x/rX) y = factor2 rX rY rZ g Hg (x/rX) y)).
-intro. do 2 rewrite factorize2. auto.
+intro. do 2 rewrite factorize2. auto using class_eq, eqv_rfl.
 Qed.
 
 (**
@@ -214,11 +184,11 @@ Section relvec.
 
   Context (A B : Type)(R : B -> B -> Prop) .
 Inductive rel_vec : forall (l : list A),
-    Vec B l -> Vec B l -> Prop :=
-  nil_rel_vec :  rel_vec  (NilV _) (NilV _)
+    vec B l -> vec B l -> Prop :=
+  nil_rel_vec :  rel_vec NilV NilV
 | cons_rel_vec : forall n l t t' v v', rel_vec (l := l)  v v' -> R t t' -> rel_vec (ConsV n t v)(ConsV n t' v').
 
-Lemma rel_vec_rfl (rx : forall x, R x x) l (v : Vec B l) : rel_vec v v.
+Lemma rel_vec_rfl (rx : forall x, R x x) l (v : vec B l) : rel_vec v v.
   induction v.
   - constructor.
   - constructor; auto.
@@ -227,12 +197,12 @@ Qed.
 
 Fixpoint vec_quot_ind
          {A B : Type}{R : Eqv B}{l : list A}
-         (P : Vec (B // R) l -> Prop)
-         (Pquot : forall (v : Vec B l), P (Vec_map (fun _ => class R) v)) 
-         (v : Vec (B // R) l) : P v.
+         (P : vec (B // R) l -> Prop)
+         (Pquot : forall (v : vec B l), P (vec_map (fun _ => class R) v)) 
+         (v : vec (B // R) l) : P v.
 Proof.
   destruct v as [|a l b v].
-  - apply (Pquot (NilV _)).
+  - apply (Pquot NilV).
   - cbn.
     revert v b.
     unshelve refine (vec_quot_ind _  _ _ _ _  _).
@@ -242,11 +212,11 @@ Proof.
        exact (fun b v => Pquot (ConsV a b v )).
 Qed.
 
-Fixpoint vec_quot_out (A B C : Type)(R : Eqv B)(l : list A)[f : Vec B l -> C]
+Fixpoint vec_quot_out (A B C : Type)(R : Eqv B)(l : list A)[f : vec B l -> C]
       (compat_f : forall b b', rel_vec R b b' -> f b = f b')
-      (v : Vec (B // R) l) : C.
+      (v : vec (B // R) l) : C.
   destruct v as [|a l b v].
-  - exact (f (NilV _)).
+  - exact (f NilV).
   - cbn.
     revert v b.
     unshelve refine (vec_quot_out _ _ _ _ _ _  _).
@@ -275,10 +245,10 @@ Fixpoint vec_quot_out (A B C : Type)(R : Eqv B)(l : list A)[f : Vec B l -> C]
       * apply eqv_rfl.
 Defined.
 
-Fixpoint vec_quot_out_proj (A B C : Type)(R : Eqv B)(l : list A)(f : Vec B l -> C)
+Fixpoint vec_quot_out_proj (A B C : Type)(R : Eqv B)(l : list A)(f : vec B l -> C)
       (compat_f : forall b b', rel_vec R b b' -> f b = f b')
-      (v : Vec B l) :
-  vec_quot_out compat_f (Vec_map (fun _ => class R) v) = f v.
+      (v : vec B l) :
+  vec_quot_out compat_f (vec_map (fun _ => class R) v) = f v.
 Proof.
   destruct v.
   - reflexivity.
